EvmEquivalence/Summaries/MstoreSummary.lean
@@ -8,8 +8,14 @@ open EvmYul.State
 
 namespace MstoreSummary
 
+inductive mstore_op where
+ | mstore
+ | mstore8
+
 section
 
+/- It's more handy to have the `op` variable at the top -/
+variable (op : mstore_op)
 variable (gas gasCost : ℕ)
 variable (symStack : Stack UInt256)
 variable (symPc symGasAvailable symRefund offset value : UInt256)
@@ -20,28 +26,64 @@ variable (symAccessedStorageKeys : Batteries.RBSet (AccountAddress × UInt256) S
 variable (symAccounts : AccountMap)
 variable (symCodeOwner : AccountAddress)
 variable (symPerm : Bool)
-
 variable (symValidJumps : Array UInt256)
 
 @[simp]
 abbrev mstoreEVM := @Operation.MSTORE .EVM
 
 @[simp]
+abbrev mstore8EVM := @Operation.MSTORE8 .EVM
+
+@[simp]
 abbrev mstore_instr : Option (Operation .EVM × Option (UInt256 × Nat)) :=
   some ⟨mstoreEVM, none⟩
 
 @[simp]
+abbrev mstore8_instr : Option (Operation .EVM × Option (UInt256 × Nat)) :=
+  some ⟨mstore8EVM, none⟩
+
+@[simp]
+def mstore_op.get : (Option (Operation .EVM × Option (UInt256 × Nat))) :=
+  match op with
+  | .mstore => mstore_instr
+  | .mstore8 => mstore8_instr
+
+def mstore_op.t : Operation OperationType.EVM :=
+  match op with
+  | .mstore => (mstore_instr.get rfl).1
+  | .mstore8 => (mstore8_instr.get rfl).1
+
+/--
+Getter for the `MachineStateOps.mstore*` function
+-/
+@[simp]
+def mstore_op.to_mso : MachineState → UInt256 → UInt256 → MachineState :=
+  match op with
+  | .mstore => EvmYul.MachineState.mstore
+  | .mstore8 => EvmYul.MachineState.mstore8
+
+@[simp]
 abbrev EVM.step_mstore : Transformer :=
-  EVM.step gas gasCost mstore_instr
+  EVM.step gas gasCost op.get
 
 @[simp]
 abbrev EvmYul.step_mstore : Transformer :=
-  EvmYul.step mstoreEVM
+  EvmYul.step op.t
+
+/--
+Different cases for the `activeWords` update
+-/
+@[simp]
+def mstore_op.to_l : ℕ :=
+  match op with
+  | .mstore => 32
+  | .mstore8 => 1
 
 /--
 Theorem needed to bypass the `private` attribute of `EVM.dispatchBinaryMachineStateOp`
  -/
-theorem mstore_bypass_private (symState : EVM.State):
+theorem mstore_bypass_private
+  (symState : EVM.State):
   let ss := {symState with
   stack := symStack,
   pc := symPc
@@ -58,21 +100,36 @@ theorem mstore_bypass_private (symState : EVM.State):
                refundBalance := symRefund}
   returnData := symReturnData,
   execLength := symExecLength}
-  EvmYul.step_mstore ss =
-  EVM.binaryMachineStateOp EvmYul.MachineState.mstore ss := rfl
+  EvmYul.step_mstore op ss =
+  EVM.binaryMachineStateOp op.to_mso ss := by cases op <;> rfl
 
 /--
 The new amount of `activeWords` based after running `MSTORE` with `offset`
 and `currentAC` amount of active words
 -/
-def activeWords_comp :=
-  UInt256.ofNat (symActiveWords.toNat ⊔ (offset.toNat + 32 + 31) / 32)
+def activeWords_comp (l : ℕ) :=
+  UInt256.ofNat (symActiveWords.toNat ⊔ (offset.toNat + l + 31) / 32)
 
 /--
 Writing `value` to `symMemory` starting at `offset`
 -/
-def mstore_memory_write :=
+def mstore_memory_write : ByteArray :=
 value.toByteArray.write 0 symMemory offset.toNat 32
+
+/--
+Writing `value` to `symMemory` starting at `offset`
+-/
+def mstore8_memory_write : ByteArray :=
+(⟨#[UInt8.ofNat value.toNat]⟩ :ByteArray).write 0 symMemory offset.toNat 1
+
+/--
+Different cases to write to memory depending on the `mstore*` opcode
+-/
+@[simp]
+def mstore_op.to_write : UInt256 → UInt256 → ByteArray → ByteArray :=
+  match op with
+  | .mstore => mstore_memory_write
+  | .mstore8 => mstore8_memory_write
 
 theorem EvmYul.step_mstore_summary (symState : EVM.State):
   let ss := {symState with
@@ -91,15 +148,16 @@ theorem EvmYul.step_mstore_summary (symState : EVM.State):
                  refundBalance := symRefund}
     returnData := symReturnData,
     execLength := symExecLength}
-  EvmYul.step_mstore ss =
+  EvmYul.step_mstore op ss =
   .ok {ss with
     stack := symStack,
     pc := symPc + .ofNat 1
-    memory := mstore_memory_write offset value symMemory,
-    activeWords := activeWords_comp offset symActiveWords} := by
-  aesop (add simp [mstore_bypass_private])
+    memory := op.to_write offset value symMemory,
+    activeWords := activeWords_comp offset symActiveWords op.to_l} := by aesop
 
-theorem EVM.step_mstore_summary (gas_pos : 0 < gas) (symState : EVM.State):
+theorem EVM.step_mstore_summary
+  (gas_pos : 0 < gas)
+  (symState : EVM.State):
   let ss := {symState with
     stack := offset :: value :: symStack,
     pc := symPc
@@ -116,62 +174,57 @@ theorem EVM.step_mstore_summary (gas_pos : 0 < gas) (symState : EVM.State):
                  refundBalance := symRefund}
     returnData := symReturnData,
     execLength := symExecLength}
-  EVM.step_mstore gas gasCost ss =
+  EVM.step_mstore op gas gasCost ss =
     .ok {ss with
           stack := symStack,
           pc := symPc + (.ofNat 1),
           gasAvailable := symGasAvailable - UInt256.ofNat gasCost,
-          memory := mstore_memory_write offset value symMemory,
-          activeWords := activeWords_comp offset symActiveWords
+          memory := op.to_write offset value symMemory,
+          activeWords := activeWords_comp offset symActiveWords op.to_l
           execLength := symExecLength + 1} := by
   cases gas; contradiction
   simp [step_mstore, EVM.step]
-  have srw := EvmYul.step_mstore_summary symStack symPc (symGasAvailable - UInt256.ofNat gasCost) symRefund offset value symActiveWords (symExecLength + 1) symReturnData symCode symMemory
-  simp [EvmYul.step_mstore, Operation.MSTORE] at srw; aesop
+  have srw := EvmYul.step_mstore_summary op symStack symPc (symGasAvailable - UInt256.ofNat gasCost) symRefund offset value symActiveWords (symExecLength + 1) symReturnData symCode symMemory
+  simp [EvmYul.step_mstore, Operation.MSTORE] at srw
+  cases op <;> aesop
+
+/--
+Opcode map to binary
+-/
+def mstore_op.to_bin : ByteArray :=
+  match op with
+  | .mstore  => ⟨#[0x52]⟩
+  | .mstore8 => ⟨#[0x53]⟩
 
 @[simp]
 theorem decode_singleton_mstore :
-  decode ⟨#[0x52]⟩ (.ofNat 0) = some ⟨mstoreEVM, none⟩ := rfl
+  decode op.to_bin (.ofNat 0) = some ⟨op.t, none⟩ := by aesop (add simp [mstore_op.t])
 
 @[simp]
 def value_and_activeWords_gas :=
-  UInt256.ofNat (MachineState.M symActiveWords.toNat value.toNat 32)
+  UInt256.ofNat (MachineState.M symActiveWords.toNat value.toNat op.to_l)
 
 @[simp]
 theorem memoryExpansionCost_mstore (symState : EVM.State)
-  (stack_ok : symState.stack = value :: symStack)
+  (stack_ok : symState.stack = offset :: value :: symStack)
   (symWords_ok : symState.activeWords = symActiveWords):
-  memoryExpansionCost symState mstoreEVM =
-  Cₘ (value_and_activeWords_gas value symActiveWords) - Cₘ symActiveWords := by
-  simp [memoryExpansionCost, memoryExpansionCost.μᵢ']
-  simp [Cₘ, stack_ok, symWords_ok]
-
-/- This theorem is incorrect, needs more constraints to have a positive
- memory expansion gas cost -/
-/-
-Memory expansion cost for the `MSTORE` opcode is strictly positive
--/
-/- theorem mec_mstore (symState : EVM.State)
-  (stack_ok : symState.stack = value :: symStack)
-  (words_ok : symState.activeWords = symActiveWords)
-  (aw_gt_0 : 0 < symActiveWords.toNat)
-  (value_big : symActiveWords.toNat < (value.toNat + 32 + 31) / 32)
-  (enough_gas : symActiveWords.toNat ⊔ (value.toNat + 32 + 31) / 32 < UInt256.size):
-  0 < memoryExpansionCost symState mstoreEVM := by
-  simp [memoryExpansionCost, Cₘ, memoryExpansionCost.μᵢ', GasConstants.Gmemory, Cₘ.QuadraticCeofficient, MachineState.M]
-  rw [UInt256.ofNat_toNat] <;> simp [words_ok, stack_ok] <;> try omega
-  apply Nat.add_lt_add
-  . aesop (add safe (by linarith))
-  . simp [max_eq_right (Nat.le_of_lt value_big)] -/
+  memoryExpansionCost symState op.t =
+  Cₘ (value_and_activeWords_gas op offset symActiveWords) -
+  Cₘ symActiveWords := by
+  cases op <;>
+  aesop (add simp [memoryExpansionCost, memoryExpansionCost.μᵢ'])
 
 theorem X_mstore_summary (symState : EVM.State)
-                         (symStack_ok : symStack.length < 1024):
+                         (symStack_ok : symStack.length <
+                         match op with
+                         | .mstore => 1024
+                         | .mstore8 => 1025):
   let ss := {symState with
     stack := offset :: value :: symStack,
     pc := .ofNat 0
     gasAvailable := symGasAvailable,
     executionEnv := {symState.executionEnv with
-                  code := ⟨#[(0x52 : UInt8)]⟩,
+                  code := op.to_bin,
                   codeOwner := symCodeOwner
                   perm := symPerm},
     accountMap := symAccounts,
@@ -183,49 +236,64 @@ theorem X_mstore_summary (symState : EVM.State)
     returnData := symReturnData,
     execLength := symExecLength}
   -- Assume we have enough gas
-  GasConstants.Gverylow < symGasAvailable.toNat - (memoryExpansionCost ss Operation.MSTORE) →
-  memoryExpansionCost ss Operation.MSTORE < UInt256.size →
+  GasConstants.Gverylow < symGasAvailable.toNat - (memoryExpansionCost ss op.t) →
+  memoryExpansionCost ss op.t < UInt256.size →
   X symGasAvailable.toNat symValidJumps ss =
   .ok (.success {ss with
           stack := symStack,
           pc := .ofNat 1,
-          gasAvailable := symGasAvailable - .ofNat (memoryExpansionCost ss mstoreEVM) - .ofNat GasConstants.Gverylow
-          memory := mstore_memory_write offset value symMemory,
-          activeWords := activeWords_comp offset symActiveWords
+          gasAvailable := symGasAvailable - .ofNat (memoryExpansionCost ss op.t) - .ofNat GasConstants.Gverylow
+          memory := op.to_write offset value symMemory,
+          activeWords := activeWords_comp offset symActiveWords op.to_l
           returnData := .empty,
           execLength := symExecLength + 2} .empty) := by
   intro ss enoughGas mec_small
-  have gavail_pos : 1 < symGasAvailable.toNat := by
+  have gavail_pos : 2 < symGasAvailable.toNat := by
     rw [GasConstants.Gverylow] at enoughGas; omega
   cases g_case : symGasAvailable.toNat; omega
   case succ g_pos =>
-  simp [X, C', δ]
+  simp [X]
   have lt_fls_rw {n m : ℕ} (_ : n < m) : (m < n) = False := by
     simp; apply Nat.ge_of_not_lt; simp; omega
-  simp [(lt_fls_rw enoughGas), α/- , (lt_fls_rw symStack_ok) -/]
-  have fls1 : (symGasAvailable.toNat < memoryExpansionCost ss (@Operation.MSTORE .EVM)) = False :=  by
+  simp [(lt_fls_rw enoughGas), α]
+  have fls1 : (symGasAvailable.toNat < memoryExpansionCost ss op.t) = False :=  by
     rw [Nat.lt_sub_iff_add_lt] at enoughGas
     aesop (add safe (by linarith))
-  have decode_rw : ((decode ss.executionEnv.code ss.pc).getD ⟨@Operation.STOP .EVM, none⟩).1 = Operation.MSTORE := rfl
+  have decode_rw : ((decode ss.executionEnv.code ss.pc).getD ⟨@Operation.STOP .EVM, none⟩).1 = op.t := by aesop
   have gavail_rw1 : ss.gasAvailable.toNat = symGasAvailable.toNat := rfl
   have gavail_rw2 : ss.gasAvailable = symGasAvailable := rfl
   simp [decode_rw, gavail_rw1, gavail_rw2, fls1]
-  simp [InstructionGasGroups.Wcopy, InstructionGasGroups.Wextaccount,
-  InstructionGasGroups.Wzero, InstructionGasGroups.Wbase, InstructionGasGroups.Wverylow]
-  have fls2 : ((symGasAvailable - UInt256.ofNat (memoryExpansionCost ss Operation.MSTORE)).toNat < GasConstants.Gverylow) = False := by
+  let Cgas := C'
+            { toState := ss.toState, gasAvailable := symGasAvailable - UInt256.ofNat (memoryExpansionCost ss op.t),
+              activeWords := ss.activeWords, memory := ss.memory, returnData := ss.returnData, H_return := ss.H_return,
+              pc := ss.pc, stack := ss.stack, execLength := ss.execLength }
+  have Cgas_rw : Cgas op.t = GasConstants.Gverylow := by
+    cases op <;> simp [Cgas, C'] <;> aesop
+  unfold Cgas at Cgas_rw
+  rw [Cgas_rw]
+  have fls2 : ((symGasAvailable - UInt256.ofNat (memoryExpansionCost ss op.t)).toNat < GasConstants.Gverylow) = False := by
     apply eq_false_intro; rw [Nat.not_lt]
     rw [UInt256.toNat_sub_dist, UInt256.ofNat_toNat] <;>
     aesop (add simp [UInt256.ofNat_le, UInt256.ofNat_toNat])
   have ss_lt2_f  (n : ℕ) : (n + 1 + 1 < 2) = False := by simp
-  simp [fls2, ss, ss_lt2_f, Nat.not_lt_of_lt symStack_ok]
-  split; contradiction
-  next state n state_ok =>
-  cases state_ok
-  have g_pos_pos : 0 < g_pos := by omega
-  have step_rw (g : UInt256) := (EVM.step_mstore_summary g_pos GasConstants.Gverylow symStack (.ofNat 0) (symGasAvailable - g) symRefund offset value symActiveWords symExecLength symReturnData ⟨#[(0x52 : UInt8)]⟩ symMemory symAccessedStorageKeys symAccounts symCodeOwner symPerm g_pos_pos symState)
-  simp [EVM.step_mstore, mstore_instr, mstoreEVM, ss] at step_rw
-  simp [step_rw, Except.instMonad, Except.bind]
-  rw [X_bad_pc] <;> aesop (add simp [GasConstants.Gverylow]) (add safe (by omega))
+  simp [fls2, ss]
+  have g_pos0 : 0 < g_pos := by omega
+  have g_pos1 : 1 < g_pos := by omega
+  have step_rw (g : UInt256) := (EVM.step_mstore_summary op g_pos GasConstants.Gverylow symStack (.ofNat 0) (symGasAvailable - g) symRefund offset value symActiveWords symExecLength symReturnData op.to_bin symMemory symAccessedStorageKeys symAccounts symCodeOwner symPerm g_pos0 symState)
+  let op_stack := match op with | .mstore => 1024 | .mstore8 => 1025
+  have : (op_stack < List.length symStack) = False := by aesop
+  cases cop : op <;> simp [δ] <;>
+  (
+    simp_all [op_stack, mstore_op.t, ss_lt2_f, this]; split
+    next _ _ h =>
+      split at h; contradiction
+      split at h; linarith
+      contradiction
+    next state n state_ok =>
+    repeat (split at state_ok; linarith)
+    cases state_ok; simp [step_rw, Except.instMonad, Except.bind]
+    rw [X_bad_pc] <;> first | linarith | congr
+  )
 
 end
 
